Iterator/Lemmas/FilterMap.lean
@@ -1,0 +1,47 @@
+/-
+Copyright (c) 2025 Lean FRO, LLC. All rights reserved.
+Released under Apache 2.0 license as described in the file LICENSE.
+Authors: Paul Reichert
+-/
+prelude
+import Iterator.Lemmas.Consumers
+import Iterator.Lemmas.Monadic.FilterMap
+import Iterator.Combinators.FilterMap
+
+theorem Iter.filterMap_eq {α β γ} [Iterator α Id β] {it : Iter (α := α) β}
+    {f : β → Option γ} :
+    it.filterMap f = (it.toIterM.filterMapH f).toPureIter :=
+  rfl
+
+theorem Iter.filterMap_step {α β γ} [Iterator α Id β] {it : Iter (α := α) β}
+    {f : β → Option γ} :
+    (it.filterMap f).step = match it.step with
+      | .yield it' out h =>
+        match h' : f out with
+        | none => .skip (it'.filterMap f) (.yieldNone (out := out) h h')
+        | some out' => .yield (it'.filterMap f) out' (.yieldSome (out := out) h h')
+      | .skip it' h => .skip (it'.filterMap f) (.skip h)
+      | .done h => .done (.done h) := by
+  simp only [filterMap_eq, step, toIterM_toPureIter, Id.run, IterM.filterMapH_stepH, Id.pure_eq,
+    Id.bind_eq]
+  generalize it.toIterM.stepH.inflate = step
+  obtain ⟨step, h⟩ := step
+  apply Subtype.ext
+  match step with
+  | .yield it' out =>
+    simp only [PlausibleIterStep.map, IterStep.map_yield, id_eq, toIterM_toPureIter,
+      PlausibleIterStep.yield, PlausibleIterStep.skip]
+    split <;> split
+    all_goals
+      simp only [USquash.inflate_deflate, IterStep.map_yield, id_eq, reduceCtorEq]
+      simp_all
+  | .skip it' =>
+    simp [PlausibleIterStep.map, IterStep.map_yield, id_eq, toIterM_toPureIter,
+      PlausibleIterStep.skip]
+  | .done =>
+    simp [PlausibleIterStep.map, PlausibleIterStep.done]
+
+  theorem Iter.toList_filterMap {α β γ} [Iterator α Id β] [IteratorToArray α Id] [LawfulIteratorToArray α Id]
+      {f : β → Option γ} {it : Iter (α := α) β} :
+      (it.filterMap f).toList = it.toList.filterMap f := by
+    simp [filterMap_eq, toList_eq_toList_toIterM, IterM.toList_filterMapH]
